make `wp` a def, fix a few simp lemmas, leave Option ones

Loom/WP/Basic.lean
@@ -13,17 +13,31 @@ variable {m : Type u → Type v}
 The WPMonad typeclass defines weakest precondition semantics for monads.
 -/
 
-class WPMonad (m : Type u → Type v) (l : outParam (Type w)) (e : outParam (Type w)) [Monad m] [CompleteLattice l] where
-  wp : m α → ECont l e α
-  wp_pure (x : α) (post : α → l) (epost : e) :
+class WPMonad (m : Type u → Type v) (l : outParam (Type w)) (e : outParam (Type w))
+    [Monad m] [CompleteLattice l] extends LawfulMonad m where
+  wpImpl : m α → ECont l e α
+  wp_pure_impl (x : α) (post : α → l) (epost : e) :
     /- TODO: put ⊑ here  -/
-    wp (pure (f := m) x) post epost = post x
-  wp_bind (x : m α) (f : α → m β) (post : β → l) (epost : e) :
-    wp x (fun x => wp (f x) post epost) epost ⊑ wp (x >>= f) post epost
-  wp_cons (x : m α) (post post' : α → l) (epost : e) (h : post ⊑ post') :
-    wp x post epost ⊑ wp x post' epost
+    wpImpl (pure (f := m) x) post epost = post x
+  wp_bind_impl (x : m α) (f : α → m β) (post : β → l) (epost : e) :
+    wpImpl x (fun x => wpImpl (f x) post epost) epost ⊑ wpImpl (x >>= f) post epost
+  wp_cons_impl (x : m α) (post post' : α → l) (epost : e) (h : post ⊑ post') :
+    wpImpl x post epost ⊑ wpImpl x post' epost
 
-export WPMonad (wp)
+def wp [Monad m] [CompleteLattice l] [WPMonad m l e] {α} (x : m α) (post : α → l) (epost : e) : l :=
+  WPMonad.wpImpl x post epost
+
+@[simp, grind =] theorem WPMonad.wp_impl_eq_wp [Monad m] [CompleteLattice l] [WPMonad m l e] {α} (x : m α):
+    WPMonad.wpImpl x = wp x := rfl
+
+theorem WPMonad.wp_pure [Monad m] [CompleteLattice l] [WPMonad m l e] (x : α) (post : α → l) (epost : e) :
+    wp (pure (f := m) x) post epost = post x := by apply wp_pure_impl
+
+theorem WPMonad.wp_bind [Monad m] [CompleteLattice l] [WPMonad m l e] (x : m α) (f : α → m β) (post : β → l) (epost : e) :
+    wp x (fun x => wp (f x) post epost) epost ⊑ wp (x >>= f) post epost := by apply wp_bind_impl
+
+theorem WPMonad.wp_cons [Monad m] [CompleteLattice l] [WPMonad m l e] (x : m α) (post post' : α → l) (epost : e) (h : post ⊑ post') :
+    wp x post epost ⊑ wp x post' epost := by apply wp_cons_impl _ _ _ _ h
 
 /-!
 # Derived theorems for WPMonad
@@ -42,6 +56,12 @@ theorem WPMonad.wp_map [Monad m] [LawfulMonad m] [CompleteLattice l] [WPMonad m 
     simp [WPMonad.wp_pure]
   rw [h]
   exact WPMonad.wp_bind x (pure ∘ f) post epost
+
+theorem WPMonad.wp_map' [Monad m] [LawfulMonad m] [CompleteLattice l] [WPMonad m l e] (f : α → β) (x : m α) :
+  ∀ post post' epost (_ : post = fun a => post' (f a)), wp x post epost ⊑ wp (f <$> x) post' epost := by
+  intro post post' epost h
+  subst h
+  apply wp_map
 
 theorem WPMonad.wp_seq [Monad m] [LawfulMonad m] [CompleteLattice l] [WPMonad m l e] (f : m (α → β)) (x : m α) :
   ∀ post epost, wp f (fun g => wp x (fun a => post (g a)) epost) epost ⊑ wp (f <*> x) post epost := by
@@ -72,85 +92,128 @@ theorem WPMonad.wp_seq [Monad m] [LawfulMonad m] [CompleteLattice l] [WPMonad m 
 -/
 
 instance Id.instWPMonad : WPMonad Id.{u} Prop Unit where
-  wp x post epost := post x
-  wp_pure x post epost := rfl
-  wp_bind x f post epost := by simp [bind]; exact PartialOrder.rel_refl
-  wp_cons x post post' epost h := by apply h
+  wpImpl x post epost := post x
+  wp_pure_impl x post epost := rfl
+  wp_bind_impl x f post epost := by simp [bind]; exact PartialOrder.rel_refl
+  wp_cons_impl x post post' epost h := by apply h
 
 -- #check Id.instWPMonad
 
 
 instance Option.instWPMonad : WPMonad Option Prop Prop where
-  wp x post epost := x.elim epost post
-  wp_pure x post epost := rfl
-  wp_bind x f post epost := by cases x <;> exact id
-  wp_cons x post post' epost h := by cases x with
+  wpImpl x post epost := x.elim epost post
+  wp_pure_impl x post epost := rfl
+  wp_bind_impl x f post epost := by cases x <;> exact id
+  wp_cons_impl x post post' epost h := by cases x with
     | none => exact id
     | some a => exact h a
 
+/--
+Adds the ability to make assertions about exceptions of type `ε` to a predicate transformer with
+postcondition shape `ps`, resulting in postcondition shape `.except ε ps`. This is done by
+interpreting `ExceptT ε (PredTrans ps) α` into `PredTrans (.except ε ps) α`.
+
+This can be used for all kinds of exception-like effects, such as early termination, by interpreting
+them as exceptions.
+-/
+/- TODO: change the order of `(e × (ε → l))` -/
+def pushExcept {α ε l e} (x : ECont l e (Except ε α)) : ECont l (e × (ε → l)) α :=
+  fun post epost => x (fun | .ok a => post a | .error e => epost.2 e) epost.1
+
+abbrev pushExcept.post {l : Type u} (post : α → l) (epost : e × (ε → l)) : Except ε α → l :=
+  fun | .ok a => post a | .error e => epost.2 e
+
+@[simp, grind =]
+theorem apply_pushExcept {α ε l e} (x : ECont l e (Except ε α)) (post : α → l) (epost : e × (ε → l)) :
+  (pushExcept x) post epost = x (pushExcept.post post epost) epost.1 := rfl
+
 /- TODO: change the order of `(e × (ε → l))` -/
 instance ExceptT.instWPMonad {l : Type u}
-  [CompleteLattice l] [Monad m] [LawfulMonad m] [WPMonad m l e] :
-  WPMonad (ExceptT ε m) l (e × (ε → l)) where
-  wp x post epost := WPMonad.wp (m := m) (l := l) (e := e) x
-    (fun | .ok x => post x | .error e => epost.2 e)
-    epost.1
-  wp_pure x post epost := by simp [pure, ExceptT.pure, ExceptT.mk, WPMonad.wp_pure]
-  wp_bind x f post epost := by
-    simp only [bind, ExceptT.bind, ExceptT.mk]
+    [CompleteLattice l] [Monad m] [LawfulMonad m] [WPMonad m l e] :
+    WPMonad (ExceptT ε m) l (e × (ε → l)) where
+  wpImpl x := pushExcept (wp x.run)
+  wp_pure_impl x post epost := by simp [WPMonad.wp_pure]
+  wp_bind_impl x f post epost := by
+    simp only [apply_pushExcept, ExceptT.run_bind]
     apply PartialOrder.rel_trans _ (WPMonad.wp_bind (m := m) x ..)
     apply WPMonad.wp_cons (m := m)
     intro r; cases r with
     | ok a => exact PartialOrder.rel_refl
-    | error _ => simp [ExceptT.bindCont, WPMonad.wp_pure (m := m)]; exact PartialOrder.rel_refl
-  wp_cons x post post' epost h := by
+    | error _ => simp [WPMonad.wp_pure (m := m)]; exact PartialOrder.rel_refl
+  wp_cons_impl x post post' epost h := by
     apply WPMonad.wp_cons
     intro r; cases r with
     | ok a => exact h a
     | error e => exact PartialOrder.rel_refl
 
+@[simp, grind =]
+theorem ExceptT.apply_wp {α ε l e} [Monad m] [CompleteLattice l] [WPMonad m l e] (x : ExceptT ε m α) (post : α → l) (epost : e × (ε → l)) :
+  (wp x) post epost = wp x.run (pushExcept.post post epost) epost.1 := rfl
+
+/--
+Adds the ability to make assertions about a state of type `σ` to a predicate transformer with
+postcondition shape `ps`, resulting in postcondition shape `.arg σ ps`. This is done by
+interpreting `StateT σ (PredTrans ps) α` into `PredTrans (.arg σ ps) α`.
+
+This can be used to for all kinds of state-like effects, including reader effects or append-only
+states, by interpreting them as states.
+-/
+-- Think: modifyGetM
+def pushArg {σ : Type u} (x : σ → ECont l e (α × σ)) : ECont (σ → l) e α :=
+  fun post epost s => x s (fun (a, s) => post a s) epost
+
+@[simp, grind =]
+theorem apply_pushArg {σ : Type u} (x : σ → ECont l e (α × σ)) (post : α → σ → l) (epost : e) (s : σ) :
+  (pushArg x) post epost s = x s (fun (a, s) => post a s) epost := rfl
+
 instance StateT.instWPMonad {l : Type u}
   [CompleteLattice l] [Monad m] [LawfulMonad m] [WPMonad m l e] :
   WPMonad (StateT σ m) (σ -> l) e where
-  wp x post epost := fun s => WPMonad.wp (m := m) (l := l) (e := e) (x s)
-    (fun x => post x.1 x.2)
-    epost
-  wp_pure x post epost := by funext s; simp [pure, StateT.pure, WPMonad.wp_pure (m := m)]
-  wp_bind x f post epost := by
+  wpImpl x := pushArg (wp ∘ x.run)
+  wp_pure_impl x post epost := by ext s; simp [WPMonad.wp_pure]
+  wp_bind_impl x f post epost := by
     intro s
-    simp only [bind, StateT.bind]
+    simp only [apply_pushArg, Function.comp_apply, StateT.run_bind]
     apply WPMonad.wp_bind
-  wp_cons x post post' epost h := by
+  wp_cons_impl x post post' epost h := by
     intro s
     apply WPMonad.wp_cons
     intro ⟨a, s'⟩
     exact h a s'
 
+@[simp, grind =]
+theorem StateT.apply_wp {σ : Type u} [Monad m] [CompleteLattice l] [WPMonad m l e] (x : StateT σ m α) (post : α → σ → l) (epost : e) (s : σ) :
+  (wp x) post epost s = wp (x.run s) (fun (a, s) => post a s) epost := rfl
+
 instance ReaderT.instWPMonad {l : Type u}
-  [CompleteLattice l] [Monad m] [LawfulMonad m] [WPMonad m l e] :
-  WPMonad (ReaderT ρ m) (ρ → l) e where
-  wp x post epost := fun r => WPMonad.wp (m := m) (l := l) (e := e) (x r)
-    (fun a => post a r)
-    epost
-  wp_pure x post epost := by funext r; simp [pure, ReaderT.pure, WPMonad.wp_pure (m := m)]
-  wp_bind x f post epost := by
+    [CompleteLattice l] [Monad m] [LawfulMonad m] [WPMonad m l e] :
+    WPMonad (ReaderT ρ m) (ρ → l) e where
+  wpImpl x := pushArg (fun r => (·, r) <$> wp (x.run r))
+  wp_pure_impl x post epost := by ext r; simp [WPMonad.wp_pure]
+  wp_bind_impl x f post epost := by
     intro r
-    simp only [bind, ReaderT.bind]
+    simp only [apply_pushArg, ECont.apply_map, ReaderT.run_bind]
     apply PartialOrder.rel_trans
     · apply WPMonad.wp_cons (m := m)
       intro a
       exact PartialOrder.rel_refl
-    · apply WPMonad.wp_bind (m := m)
-  wp_cons x post post' epost h := by
+    · apply WPMonad.wp_bind
+  wp_cons_impl x post post' epost h := by
     intro r
     apply WPMonad.wp_cons (m := m)
     intro a
     exact h a r
 
+@[simp, grind =]
+theorem ReaderT.apply_wp {ρ : Type u} [Monad m] [CompleteLattice l] [WPMonad m l e] (x : ReaderT ρ m α) (post : α → ρ → l) (epost : e) (r : ρ) :
+  (wp x) post epost r = wp (x.run r) (fun a => post a r) epost := rfl
+
+/-
+TODO: Same as for pushExcept
 instance OptionT.instWPMonad {l : Type u}
   [CompleteLattice l] [Monad m] [LawfulMonad m] [WPMonad m l e] :
   WPMonad (OptionT m) l (e × l) where
-  wp x post epost := WPMonad.wp (m := m) (l := l) (e := e) x.run
+  wpImpl x post epost := WPMonad.wp (m := m) (l := l) (e := e) x.run
     (fun o => match o with | some a => post a | none => epost.2)
     epost.1
   wp_pure x post epost := by
@@ -168,6 +231,7 @@ instance OptionT.instWPMonad {l : Type u}
     cases o with
     | some a => exact h a
     | none => exact PartialOrder.rel_refl
+-/
 
 /-!
 # Type alias instances
@@ -182,33 +246,33 @@ instance Reader.instWPMonad : WPMonad (ReaderM ρ) (ρ → Prop) PUnit :=
 
 -- Except is a simple sum type, so error continuation is just ε → Prop
 instance Except.instWPMonad : WPMonad (Except ε) Prop (PUnit × (ε → Prop)) where
-  wp x post epost := match x with
+  wpImpl x post epost := match x with
     | .ok a => post a
     | .error e => epost.2 e
-  wp_pure x post epost := rfl
-  wp_bind x f post epost := by cases x <;> exact id
-  wp_cons x post post' epost h := by cases x with
+  wp_pure_impl x post epost := rfl
+  wp_bind_impl x f post epost := by cases x <;> exact id
+  wp_cons_impl x post post' epost h := by cases x with
     | ok a => exact h a
     | error e => exact id
 
 -- EStateM combines state and exceptions
 instance EStateM.instWPMonad : WPMonad (EStateM ε σ) (σ → Prop) (ε → σ → Prop) where
-  wp x post epost := fun s => match x s with
+  wpImpl x post epost := fun s => match x s with
     | .ok a s' => post a s'
     | .error e s' => epost e s'
-  wp_pure x post epost := by
+  wp_pure_impl x post epost := by
     funext s
-    simp [pure, EStateM.pure]
-  wp_bind x f post epost := by
+    simp [wp, pure, EStateM.pure]
+  wp_bind_impl x f post epost := by
     intro s
-    simp only [bind, EStateM.bind]
+    simp only [wp, bind, EStateM.bind]
     cases (x s) <;> exact PartialOrder.rel_refl
-  wp_cons x post post' epost h := by
+  wp_cons_impl x post post' epost h := by
     intro s
     generalize heq : x s = r
     cases r with
-    | ok a s' => simp [heq]; exact h a s'
-    | error e s' => simp [heq]; exact PartialOrder.rel_refl
+    | ok a s' => simp [wp, heq]; exact h a s'
+    | error e s' => simp [wp, heq]; exact PartialOrder.rel_refl
 
 /-!
 # Adequacy lemmas
@@ -258,7 +322,7 @@ theorem EStateM.of_wp_run_eq {ε σ α : Type} {x : EStateM.Result ε σ α} {pr
   (h : EStateM.run prog s = x) (P : EStateM.Result ε σ α → Prop)
   (hwp : wp prog (fun a s' => P (.ok a s')) (fun e s' => P (.error e s')) s) : P x := by
   rw [← h]
-  simp only [wp] at hwp
+  simp [wp, WPMonad.wpImpl] at hwp -- TODO: Probably should define a simp lemma for impl of `wp`
   change P (prog s)
   cases heq : prog s with
   | ok a s' => simp [heq] at hwp; exact hwp
